importing new C code to verify from RL-Put-Cursor branch. adapt VST proofs

verif/relation_mem.c
@@ -11,7 +11,7 @@
  * Created on September 23, 2017, 7:31 PM
  */
 
-/* #include "relation.h" */
+#include "relation.h"
 #include <assert.h>
 /* #include <stdlib.h> */
 #include <string.h>
@@ -22,18 +22,6 @@
 extern void free (void *);
 extern void * malloc (unsigned int n);
 
-/* util.h */
-typedef enum { False = 0 , True = 1} Bool;
-enum {FANOUT = 15};
-enum {MAX_TREE_DEPTH = 20};
-size_t UTIL_Min(size_t a, size_t b);
-Bool UTIL_StrEqual(const char* a, size_t lenA, const char* b, size_t lenB);
-
-/* relation.h */
-typedef struct Relation* Relation_T;
-typedef struct Cursor* Cursor_T;
-
-
 /* Type declarations */
 typedef struct BtNode BtNode;
 typedef struct Entry Entry;
@@ -41,11 +29,13 @@ typedef union Child_or_Record Child_or_Record;
 typedef struct Cursor Cursor;
 
 /* Function Declarations */
-static BtNode* createNewNode(Bool isLeaf);
+static BtNode* createNewNode(Bool isLeaf, Bool FirstLeaf, Bool LastLeaf);
 
-static Bool insertKeyRecord(BtNode* node, unsigned long key, const void* record,
-        Entry * const newEntryFromChild, Cursor* cursor, Relation_T relation,
-        const int level);
+static void goToKey(Cursor_T cursor, unsigned long key);
+
+static Bool isNodeParent(BtNode * currNode, unsigned long key);
+
+static void putEntry(Cursor_T cursor,int level, Entry * newEntry, size_t key);
 
 static Bool deleteKeyRecord(BtNode* parentNode, BtNode* node, unsigned long key,
         Entry* const oldEntryFromChild, Cursor* cursor, Relation_T relation, 
@@ -60,10 +50,16 @@ static void redistributeOrMerge(BtNode* leftNode, BtNode* rightNode,
 
 static int findChildIndex(const Entry* entries, unsigned long key, int length);
 
-static Bool moveToRecord(BtNode* node, unsigned long key, Cursor* cursor, 
-        const int level, int *pRes);
+static int findRecordIndex(const Entry* entries, unsigned long key, int length);
 
-static Bool moveToFirstRecord(BtNode* node, Cursor* cursor, int level);
+static void moveToKey(BtNode* node, unsigned long key, Cursor* cursor,
+	const int level);
+
+static void moveToNext(Cursor_T cursor);
+
+static void moveToFirst(BtNode* node, Cursor* cursor, int level);
+
+static void moveToLast(BtNode* node, Cursor* cursor, int level);
 
 static void handleDeleteBtree(BtNode* node, void (* freeRecord)(void *));
 
@@ -71,6 +67,7 @@ static void ASSERT_NODE_INVARIANT(BtNode* node, Relation_T relation);
 
 static void printTree(BtNode* node, int level);
 
+static void printCursor(Cursor_T cursor);
 
 
 /**********************************
@@ -89,6 +86,7 @@ typedef struct Relation {
     /* Root node of btree */
     struct BtNode* root;
     size_t numRecords;
+    int depth;
 } Relation;
 
 /* Each entry in a btree node has a key. 
@@ -111,6 +109,10 @@ struct Entry {
 struct BtNode {
     /* Is this a leaf?*/
     Bool isLeaf;
+    /* Is this the first Leaf */
+    Bool FirstLeaf;
+    /* Is this the last Leaf */
+    Bool LastLeaf;
     /* Current number of keys in the node */
     int numKeys;
     /* Ptr to first child */
@@ -125,23 +127,41 @@ struct BtNode {
 struct Cursor {
     /* The relation that this cursor points to*/
     Relation* relation;
-    /* The current Node BtCursor is pointing to */
-    BtNode* currNode;
-    /* The index of the entry in currNode, BtCursor is pointing to. */
-    size_t entryIndex;
-    /* Is this Cursor valid? */
-    Bool isValid;
     /*What level is the cursor at*/
     int level;
     /* Arrays of index at ancestor node[i] containing child pointer to next 
      * ancestor node [i + 1]. */
     /* indices range from -1 to NUM_KEYS - 1. At leaf, index is entryIdx */
-    int nextAncestorPointerIdx[MAX_TREE_DEPTH];
+    int ancestorsIdx[MAX_TREE_DEPTH];
     /* Array of Current Nodes Ancestors*/
     BtNode* ancestors[MAX_TREE_DEPTH];
 };
 
-/* TODO: set cursor method */
+int entryIndex (Cursor_T cursor) {
+  return cursor->ancestorsIdx[cursor->level];
+}
+
+BtNode* currNode (Cursor_T cursor) {
+  return cursor->ancestors[cursor->level];
+}
+
+Bool isValid (Cursor_T cursor) {
+  if (entryIndex(cursor) == currNode(cursor)->numKeys &&
+      currNode(cursor)->LastLeaf == True) {
+    return False;
+  } else {
+    return True;
+  }
+}
+
+Bool isFirst (Cursor_T cursor) {
+  if (entryIndex(cursor) == 0 &&
+      currNode(cursor)->FirstLeaf == True) {
+    return True;
+  } else {
+    return False;
+  }
+}
 
 /**********************************
  * Function Definitions           *
@@ -151,7 +171,7 @@ Relation_T RL_NewRelation(void) {
     BtNode* pRootNode;
     Relation* pNewRelation;
 
-    pRootNode = createNewNode(True);
+    pRootNode = createNewNode(True, True, True);
     if (pRootNode == NULL) {
         return NULL;
     }
@@ -164,7 +184,8 @@ Relation_T RL_NewRelation(void) {
 
     pNewRelation->root = pRootNode;
     pNewRelation->numRecords = 0;
-
+    pNewRelation->depth = 0;
+    
     return pNewRelation;
 }
 
@@ -176,7 +197,7 @@ void RL_DeleteRelation(Relation_T relation, void (* freeRecord)(void *)){
 
 Cursor_T RL_NewCursor(Relation_T relation) {
     Cursor* cursor;
-    int i;
+    size_t i;
 
     assert(relation != NULL);
 
@@ -186,13 +207,10 @@ Cursor_T RL_NewCursor(Relation_T relation) {
     }
 
     cursor->relation = relation;
-    cursor->currNode = NULL;
-    cursor->entryIndex = 0;
-    cursor->isValid = False;
     cursor->level = 0;
-
-    for (i = 0; i < MAX_TREE_DEPTH; i++) {
-        cursor->nextAncestorPointerIdx[i] = 0;
+    moveToFirst(relation->root, cursor, 0);
+    for (i = cursor->level+1; i < MAX_TREE_DEPTH; i++) {
+        cursor->ancestorsIdx[i] = 0;
         cursor->ancestors[i] = NULL;
     }
     return cursor;
@@ -204,213 +222,258 @@ void RL_FreeCursor(Cursor_T btCursor) {
 
 Bool RL_CursorIsValid(Cursor_T cursor) {
     assert(cursor != NULL);
-    return cursor->isValid;
+    return isValid(cursor);
 }
 
-Bool RL_PutRecord(Cursor_T cursor, unsigned long key, const void* record) {
-    Bool success;
-    Entry newEntryFromChild;
+void RL_PutRecord(Cursor_T cursor, unsigned long key, const void* record) {
+    Entry newEntry;
     assert(cursor != NULL);
 
-    newEntryFromChild.ptr.child = NULL;
+    newEntry.ptr.record = record;
+    newEntry.key = key;
 
-    success = insertKeyRecord(cursor->relation->root, key, record,
-            &newEntryFromChild, cursor, cursor->relation, 0);
+    goToKey(cursor,key);
+    putEntry(cursor,cursor->level, &newEntry, key);
+    RL_MoveToNext(cursor);
+    
+    return;
+}
 
-    /*TODO: move cursor->isValid = True etc. into return statement here. */
-    if (success) {
-        return success;
-    }
+/* Returns true if we know for sure that currNode (Intern Node) is a parent of the key
+ * Returns False if we can't know */
+static Bool isNodeParent (BtNode * currNode, unsigned long key) {
 
-    cursor->isValid = False;
+  int idx;
+  idx = findChildIndex(currNode->entries, key, currNode->numKeys);
+  if (idx == -1 || idx == currNode->numKeys -1) {
     return False;
+  }
+  return True;
+
 }
 
-Bool RL_MoveToRecord(Cursor_T cursor, unsigned long key, int *pRes) {
-    unsigned long lowest, highest;
-    assert(cursor != NULL);
+/* Go up in the cursor until we are sure to be in a parent node of the key */
+void AscendToParent (Cursor_T cursor, unsigned long key) {
+  unsigned long lowest, highest;
 
+  if (cursor->level == 0) {/* if we are at the root */
+    return;
+  }
 
-    if (cursor->isValid) {
-        lowest = cursor->currNode->entries[0].key;
-        highest = cursor->currNode->entries[cursor->currNode->numKeys - 1].key;
-        if (key >= lowest && key <= highest) {
-            return moveToRecord(cursor->currNode, key, cursor, cursor->level, pRes);
-        }
+  if (currNode(cursor)->isLeaf) { /* current node is leaf node */
+    /* we first check if the cursor should point to the same leaf node */
+    lowest = currNode(cursor)->entries[0].key;
+    highest = currNode(cursor)->entries[currNode(cursor)->numKeys - 1].key;
+
+    if ((key >= lowest && key <= highest) ||
+	(key >= lowest && currNode(cursor)->LastLeaf == True) ||
+	(key <= highest && currNode(cursor)->FirstLeaf == True)) {
+      return;
     }
-        return moveToRecord(cursor->relation->root, key, cursor, 0, pRes);
-        
+
+    /* Else, we should move up one level */
+    cursor->level --;
+    AscendToParent(cursor, key);
+    return;
+
+  } else { /* current node is intern node */
+    if (isNodeParent(currNode(cursor), key) == True) {
+      return;
+    }
+    else {
+      cursor->level --;
+      AscendToParent(cursor, key);
+      return;
+    }
+  }
 }
 
 const void* RL_GetRecord(Cursor_T cursor) {
-    assert(cursor->isValid);
-    return (cursor->currNode->entries)[cursor->entryIndex].ptr.record;
-}
+  assert(isValid(cursor) == True);
 
-
-Bool RL_DeleteRecord(Cursor_T cursor, unsigned long key) {
-    Bool success;
-    Entry oldEntryFromChild;
-    assert(cursor != NULL);
-
-    oldEntryFromChild.ptr.child = NULL;
-
-    success = deleteKeyRecord(NULL, cursor->relation->root, key,
-            &oldEntryFromChild, cursor, cursor->relation, 0);
-
-    /*TODO: move cursor->isValid = True, etc into return statement here. */
-    if (success) {
-        cursor->isValid = False;
-        cursor->relation->numRecords--;
-        return success;
-    }
-
-    cursor->isValid = False;
-    return False;
-}
-
-
-Bool RL_MoveToFirstRecord(Cursor_T btCursor) {
-    
-    Bool success;
-    
-    assert(btCursor);
-    
-    success = moveToFirstRecord(btCursor->relation->root, btCursor, 0);
-    btCursor->isValid = success;
-    return success;
-     
-    
-}
-
-Bool RL_MoveToNext(Cursor_T btCursor) {
-        
-    int numKeys, currLevel, newIdx;
-    numKeys = btCursor->currNode->numKeys;
-    currLevel = btCursor->level;
-        
-    assert(btCursor != NULL);
-    assert(btCursor->isValid);
-    
-    /* If cursor is not at last index, set it to next index.*/
-    if(btCursor->entryIndex < (size_t)(numKeys - 1)) {
-        btCursor->entryIndex++;
-        btCursor->nextAncestorPointerIdx[currLevel] = btCursor->entryIndex;
-        btCursor->isValid = True;
-        return True;
-    }
-    
-    /* While below root and ancestor pointer is last pointer, ascend. */
-    while(currLevel >= 0 && (btCursor->nextAncestorPointerIdx[currLevel] == 
-            btCursor->ancestors[currLevel]->numKeys - 1)){
-        currLevel--;
-    }
-
-    
-    /* If at last record, currLevel would be at root.*/
-    if (currLevel < 0) {
-        return False;
-    }
-    
-    /* Go down next child to next level */
-    newIdx = ++(btCursor->nextAncestorPointerIdx[currLevel]);
-    btCursor->ancestors[currLevel+1] = btCursor->ancestors[currLevel]->entries[newIdx].ptr.child;
-    currLevel++;
-    
-    /* Descend to correct leaf down leftmost child. All leaves have same level. */
-    while(currLevel < btCursor->level){
-        btCursor->nextAncestorPointerIdx[currLevel] = -1;
-        btCursor->ancestors[currLevel+1] = btCursor->ancestors[currLevel]->entries[-1].ptr.child;
-        currLevel++; 
-    }
-    
-    btCursor->currNode = btCursor->ancestors[currLevel];
-    btCursor->nextAncestorPointerIdx[currLevel] = 0;
-    btCursor->entryIndex = 0;
-    btCursor->isValid = True;
-    
-    return True; 
-}
-
-
-Bool RL_MoveToPrevious(Cursor_T btCursor) {
-    
-    int numKeys, currLevel, newIdx;
-    numKeys = btCursor->currNode->numKeys;
-    currLevel = btCursor->level;
-        
-    assert(btCursor != NULL);
-    assert(btCursor->isValid);
-    
-    /* If cursor is not at last index, set it to previous index.*/
-    if(btCursor->entryIndex > (size_t) 0 ) {
-        btCursor->entryIndex--;
-        btCursor->nextAncestorPointerIdx[currLevel] = btCursor->entryIndex;
-        btCursor->isValid = True;
-        return True;
-    } else {
-        /* We are in leftmost entry of leaf. There is no entry -1. Go up a level. */
-        currLevel--;
-    }
-    
-    /* While below root and ancestor pointer is first pointer, ascend. */
-    while(currLevel >= 0 && (btCursor->nextAncestorPointerIdx[currLevel] == -1)){
-        currLevel--;
-    }
-
-    
-    /* If at last record, currLevel would be at root.*/
-    if (currLevel < 0) {
-        return False;
-    }
-    
-    /* Go down previous child to next (lower) level */
-    newIdx = --(btCursor->nextAncestorPointerIdx[currLevel]);
-    btCursor->ancestors[currLevel+1] = btCursor->ancestors[currLevel]->entries[newIdx].ptr.child;
-    currLevel++;
-    
-    /* Descend to correct leaf down rightmost child. All leaves have same level. */
-    while(currLevel < btCursor->level){
-        int lastIdx = btCursor->ancestors[currLevel]->numKeys - 1;
-        
-        btCursor->nextAncestorPointerIdx[currLevel] = lastIdx;
-        btCursor->ancestors[currLevel+1] = btCursor->ancestors[currLevel]->entries[lastIdx].ptr.child;
-        currLevel++; 
-    }
-    
-    numKeys = btCursor->ancestors[currLevel]->numKeys;
-
-    btCursor->currNode = btCursor->ancestors[currLevel];    
-    btCursor->nextAncestorPointerIdx[currLevel] = 0;
-    btCursor->entryIndex = numKeys - 1;
-    btCursor->isValid = True;
-    
-    return True; 
+  /* if the cursor is at the last position of a leaf node, we move to the equivalent position */
+  if (entryIndex(cursor) == currNode(cursor)->numKeys) {
+    moveToNext(cursor);
+  }
+  
+  return (currNode(cursor)->entries)[entryIndex(cursor)].ptr.record;
 }
 
 unsigned long RL_GetKey(Cursor_T cursor) {
-    assert(cursor != NULL);
-    assert(cursor->isValid);
+    assert(isValid(cursor)==True);
+
+    /* if the cursor is at the last position of a leaf node, we move to the equivalent position */
+    if (entryIndex(cursor) == currNode(cursor)->numKeys) {
+      moveToNext(cursor);
+    }
     
-    return cursor->currNode->entries[cursor->entryIndex].key;
+    return currNode(cursor)->entries[entryIndex(cursor)].key;
+}
+
+void goToKey(Cursor_T cursor, unsigned long key) {
+  assert(cursor != NULL);
+  AscendToParent(cursor, key);
+  moveToKey(currNode(cursor), key, cursor, cursor->level);
+}
+
+Bool RL_MoveToKey(Cursor_T cursor, unsigned long key) {
+    goToKey(cursor,key);
+    
+    if (isValid(cursor) == False) {
+      return False;
+    }
+    if (RL_GetKey(cursor) == key) {
+      return True;
+    } else {
+      return False;
+    } 
+}
+
+Bool RL_DeleteRecord(Cursor_T cursor, unsigned long key) {
+    /* Bool success; */
+    /* Entry oldEntryFromChild; */
+    /* assert(cursor != NULL); */
+
+    /* oldEntryFromChild.ptr.child = NULL; */
+
+    /* success = deleteKeyRecord(NULL, cursor->relation->root, key, */
+    /*         &oldEntryFromChild, cursor, cursor->relation, 0); */
+
+    /* /\*TODO: move cursor->isValid = True, etc into return statement here. *\/ */
+    /* if (success) { */
+    /*     isValid(cursor) = False; */
+    /*     cursor->relation->numRecords--; */
+    /*     return success; */
+    /* } */
+
+    /* cursor->isValid = False; */
+    return False;
+}
+
+Bool RL_MoveToFirst(Cursor_T cursor) {  
+    assert(cursor);
+    
+    moveToFirst(cursor->relation->root, cursor, 0);
+    return isValid(cursor);
 }
 
 
-Bool RL_IsEmpty(Cursor_T btCursor) {
-    BtNode* root;
-    assert(btCursor != NULL);
+int lastpointer(Bool isLeaf, int numKeys) {
+  if (isLeaf == True) {
+    return numKeys;
+  } else {
+    return numKeys-1;
+  }
+}
+
+int firstpointer(Bool isLeaf) {
+  if (isLeaf == True) {
+    return 0;
+  } else {
+    return -1;
+  }
+}
+
+/* Moves the cursor to the next position */
+static void moveToNext(Cursor_T cursor) {
+  /* If the btree is empty, return. */
+  if(cursor->relation->numRecords == 0) {
+    return;
+  }
     
-    root = btCursor->relation->root;
-    if (root->isLeaf && root->numKeys == 0) {
+  /* If past last element, stay past element and return. */
+  if(isValid(cursor) == False) {
+    return;
+  }
+        
+  /* While ancestor pointer is last pointer, ascend. */
+  while(cursor->level > 0 && entryIndex(cursor) == lastpointer(currNode(cursor)->isLeaf,currNode(cursor)->numKeys)) {
+        cursor->level--;
+  }
+
+  /* Increase index */
+  cursor->ancestorsIdx[cursor->level] ++;
+  
+  if(currNode(cursor)->isLeaf == True) {
+    return;
+  }
+
+  moveToFirst(currNode(cursor)->entries[entryIndex(cursor)].ptr.child, cursor, cursor->level+1);
+  return;
+}
+
+static void moveToPrev(Cursor_T cursor) {
+  /* If the btree is empty, return. */
+  if (cursor->relation->numRecords == 0) {
+    return;
+  }
+
+  /* If first cursor, stay first cursor and return */
+  if(isFirst(cursor) == True) {
+    return;
+  }
+
+  /* While ancestor pointer is first pointer, ascend */
+  while(cursor->level > 0 && entryIndex(cursor) == firstpointer(currNode(cursor)->isLeaf)) {
+    cursor->level--;
+  }
+
+  /* Decrease Index */
+  cursor->ancestorsIdx[cursor->level] ++;
+
+  if(currNode(cursor)->isLeaf == True) {
+    return;
+  }
+
+  moveToLast(currNode(cursor)->entries[entryIndex(cursor)].ptr.child, cursor, cursor->level+1);
+  return;
+}
+
+void RL_MoveToNext(Cursor_T cursor) {
+  
+  /* if we are at the end of a leaf, we must move to next position twice */
+  if (entryIndex(cursor) == currNode(cursor)->numKeys) {
+    moveToNext(cursor);
+  }
+  moveToNext(cursor);
+  return;
+ }
+
+void RL_MoveToPrevious(Cursor_T cursor) {
+  if (entryIndex(cursor) == 0) {
+    moveToPrev(cursor);
+  }
+  moveToPrev(cursor);
+  return;
+}
+
+Bool RL_MoveToNextValid(Cursor_T cursor) {
+  RL_MoveToNext(cursor);
+  return RL_CursorIsValid(cursor);
+}
+
+Bool RL_MoveToPreviousNotFirst(Cursor_T cursor) {
+  RL_MoveToPrevious(cursor);
+  if (isFirst(cursor) == True) {
+    return False;
+  } else {
+    return True;
+  }
+}
+
+Bool RL_IsEmpty(Cursor_T cursor) {
+    assert(cursor != NULL);
+    
+    if (cursor->relation->root->numKeys == 0) {
         return True;
     }
     return False;
 }
 
-size_t RL_NumRecords(Cursor_T btCursor) {
-    assert(btCursor != NULL);
+size_t RL_NumRecords(Cursor_T cursor) {
+    assert(cursor != NULL);
     
-    return btCursor->relation->numRecords;
+    return cursor->relation->numRecords;
     
 }
 
@@ -423,10 +486,16 @@ void RL_PrintTree(Relation_T relation) {
     
 }
 
+void RL_PrintCursor(Cursor_T cursor) {
+
+  assert (cursor != NULL);
+
+  printCursor(cursor);
+
+}
 
 
-
-static BtNode* createNewNode(Bool isLeaf) {
+static BtNode* createNewNode(Bool isLeaf, Bool FirstLeaf, Bool LastLeaf) {
     BtNode* newNode;
 
     newNode = (BtNode*) malloc(sizeof (BtNode));
@@ -436,416 +505,184 @@ static BtNode* createNewNode(Bool isLeaf) {
 
     newNode->numKeys = 0;
     newNode->isLeaf = isLeaf;
+    newNode->FirstLeaf = FirstLeaf;
+    newNode->LastLeaf = LastLeaf;
     newNode->ptr0 = NULL;
 
     return newNode;
 }
 
-/* Algorithm from page 259 of Database Management Systems Second Edition. 
- * Insert (update) key and record into leaf in nodePtr. Use newEntryFromChild to detect if a 
- * split has occurred. It is a constant pointer to an entry. It should be filled
- * in with the correct value. It contains a middle key from split and a pointer 
- * to the second node resulting from the split.  Let cursor point to newly 
- * created record. 
- * 
- * Return True on success. Return False on failure. */
-static Bool insertKeyRecord(BtNode* node, unsigned long key, const void* record,
-        Entry * const newEntryFromChild, Cursor* cursor, Relation_T relation,
-        const int level){
-    Bool success;
-    /* Index of pointer to child tree containing inserted key */
-    int childTreePtrIdx;
+/* Insert entry and split node. Return a new entry to be inserted in parent. 
+ * If this is a leaf node, new entry's key is a copy of the first key to
+ * in the second node. Otherwise, newEntry's key is the key between the last key
+ * of the first node and the first key of the second node. In both cases ptr is 
+ * a ptr to the newly created node. */
+static Entry* splitnode(BtNode* node, Entry* entry, Bool isLeaf) {
+    Entry allEntries[FANOUT + 1];
+    Entry* newEntry;
+    BtNode* newNode;
+    int i, j, tgtIdx, startIdx;
+    Bool inserted;
+    int middle;
 
-    assert(node != NULL);
-    assert(cursor != NULL);
-    /* Container to store new entry should never be NULL.*/
-    assert(newEntryFromChild != NULL);
-    assert(level < MAX_TREE_DEPTH);
+    middle = (FANOUT+1) / 2;
     
-    ASSERT_NODE_INVARIANT(node, relation);
-
-    /* Assign current node as ancestor node at current level */
-    cursor->ancestors[level] = node;
-
-    /* If node is non-leaf node*/
-    if (node->isLeaf == False) {
-        BtNode* childNode;
-        childTreePtrIdx = findChildIndex(node->entries, key,
-                node->numKeys);
-
-        if (childTreePtrIdx == -1) {
-            childNode = node->ptr0;
-        } else {
-            childNode = node->entries[childTreePtrIdx].ptr.child;
-        }
+    /* Find first key that is greater than search key. Search key goes before this key. */
+    /* Question: is this correct node? */
+    tgtIdx = findRecordIndex(node->entries, entry->key, node->numKeys);
     
-        /* set index of pointer in current node that leads to next ancestor */
-        cursor->nextAncestorPointerIdx[level] = childTreePtrIdx;
-        
-        success = insertKeyRecord(childNode, key,
-                record, newEntryFromChild, cursor, relation, level + 1);
-
-        /* if insert failed, return that insert failed */
-        if (success == False) {
-            return False;
+    j = 0;
+    inserted = False;
+    
+    /* Build list of all entries. */
+    for(i = 0; i < FANOUT + 1; i++) {  
+        if(inserted == False && j == tgtIdx) {
+            allEntries[i] = *entry;
+            inserted = True;
+            continue;
         }
-        /*  else if successful and no split, return success.*/
-        if (newEntryFromChild->ptr.child == NULL) {
-            return success;
-        }
-
-
-        /* If enough space to insert newChildEntry, insert it */
-        if (node->numKeys < FANOUT) {
-            size_t i;
-            unsigned long newKey = newEntryFromChild->key;
-
-            /* Find first entry which newEntry is greater than or equal to
-             * child goes to the right of this index. */
-            const size_t targetIdx = findChildIndex(node->entries, newKey, node->numKeys);
-                        
-            
-            /* Move all entries to the right of childIndex one to the right*/
-            for (i = node->numKeys; i > targetIdx + 1; i--) {
-                /* move keys and pointers to the right */
-                node->entries[i] = node->entries[i - 1];
-            }
-            node->entries[targetIdx + 1] = *newEntryFromChild;
-            node->numKeys++;
-            
-            /* if key is greater than or equal to new entry from child record in
-             * subtree pointed to by newEntryFromChild->child
-             */
-            if (key >= newKey) {
-                cursor->nextAncestorPointerIdx[level] = targetIdx + 1;
-            }
-            
-
-            newEntryFromChild->ptr.child = NULL;
-
-            return True;
-        }
-            /* Else split node. We have FANOUT + 1 keys and FANOUT + 2 pointers.
-             * Keep first d (floor of FANOUT / 2) keys in the first Node with d+1
-             * pointers. Set d+1 key to newEntryFromChild. Move the rest to second node.
-             * Set pointer to second node in newEntryFromChild. 
-             * If the node is the root, create a new root node from child entry and 
-             * let it point to both nodes from split. */
-        else {
-            /* Create an Array that can hold all entries. */
-            Entry allEntries[FANOUT + 1];
-            BtNode* newNode;
-            int i, j, newChildIdxAllEntries;
-            int newEntryIdx = FANOUT / 2;
-            /* index of first key that new Key is greater than or equal to  */
-            const int newTargetIdx = findChildIndex(node->entries,
-                    newEntryFromChild->key, node->numKeys);
-
-            /* To make code simpler, we will store address of child node that
-             * record was inserted into. Use this to make it easier to track 
-             * which node subtree child is in */
-            BtNode* childNode;
-            /* If key is smaller than new entry from child, 
-             * record inserted in old child tree*/
-            if (key < newEntryFromChild->key) {
-                if (childTreePtrIdx == -1) {
-                    childNode = node->ptr0;
-                }
-                else {
-                    childNode = node->entries[childTreePtrIdx].ptr.child;
-                }  
-            }
-            /* Else record inserted in new child's tree */
-            else {
-                childNode = newEntryFromChild->ptr.child;
-            }
-            
-            /* copy 0 to targetIdx of node's keys to allEntries, insert 
-             * newKeyFromChild, copy remaining targetIdx to MAXNUMKEYS - 1 
-             * keys to allEntries. Find index of subtree record was inserted to,
-             */
-            j = 0, newChildIdxAllEntries = -1;
-            for (i = 0; i < FANOUT + 1; i++) {
-                if (i == (int) newTargetIdx + 1) {
-                    allEntries[i] = *newEntryFromChild;
-                    
-                } else {
-                    allEntries[i] = node->entries[j];
-                    j++;
-                }
-                if (allEntries[i].ptr.child == childNode) {
-                    newChildIdxAllEntries = i;
-                }   
-            }
-
-            /* overwrite current node with floor of first half of keys and 
-             * pointers. 
-             * TODO: Optimize later! Unnecessary copying over.
-             */
-            for (i = 0; i < newEntryIdx; i++) {
-                node->entries[i] = allEntries[i];
-            }
-            node->numKeys = newEntryIdx;
-
-            /* create a new non-leaf node to contain second half (not including entry at 
-             * newEntryIdx) of split key.
-             * copy them to new node */
-            newNode = createNewNode(False);
-            /* TODO: handle memory error better*/
-            assert(newNode);
-
-            j = 0;
-            for (i = newEntryIdx + 1; i < FANOUT + 1; i++) {
-                newNode->entries[j] = allEntries[i];
-                j++;
-            }
-            newNode->numKeys = j;
-            newNode->ptr0 = allEntries[newEntryIdx].ptr.child;
-
-            /*Set newEntryFromChild*/
-            newEntryFromChild->key = allEntries[newEntryIdx].key;
-            newEntryFromChild->ptr.child = newNode;
-
-            /* set ancestor node and next ancestor pointer depending on 
-             * location of pointer to child subtree containing inserted record. 
-             * Setting ancestors[level] might be unnecessary in some cases where
-             * child subtree containing record does not change after split. */
-            if (newChildIdxAllEntries < newEntryIdx) {
-                cursor->ancestors[level] = node;
-                cursor->nextAncestorPointerIdx[level] = newChildIdxAllEntries;
-            }
-            else {
-                cursor->ancestors[level] = newNode;
-                cursor->nextAncestorPointerIdx[level] = newChildIdxAllEntries - 
-                        (newEntryIdx + 1);
-            }
-            
-
-            /* If this is the root level, create new root, let it point to this node and
-             * new Child entry. */
-            if (relation->root == node) {
-                BtNode* newRootNode = createNewNode(False);
-                int i;
-                assert(newRootNode);
-
-                newRootNode->ptr0 = node;
-                newRootNode->numKeys = 1;
-                newRootNode->entries[0] = *newEntryFromChild;
-
-                relation->root = newRootNode;
-
-                newEntryFromChild->ptr.child = NULL;
-                
-                /* new level created */
-                for(i = cursor->level + 1; i > 0; i--){
-                    cursor->ancestors[i] = cursor->ancestors[i-1];
-                    cursor->nextAncestorPointerIdx[i] = 
-                            cursor->nextAncestorPointerIdx[i-1];
-                }
-                
-                cursor->ancestors[0] = relation->root;
-                if (key < newEntryFromChild->key) {
-                    cursor->nextAncestorPointerIdx[0] = -1;
-                } else {
-                    cursor->nextAncestorPointerIdx[0] = 0;
-                }
-                
-                cursor->level++;
-            }
-            return True;
-        }
-    }        
-    /* If node is leaf node. */
-    else {
-        int targetIdx;
-        /* If first key, insert record and return success*/
-        if (node->numKeys == 0) {
-            node->entries[0].key = key;
-            node->entries[0].ptr.record = record;
-            node->numKeys++;
-
-            cursor->currNode = node;
-            cursor->entryIndex = 0;
-            cursor->isValid = True;
-            cursor->relation->numRecords++;
-            
-            /*Set index of pointer in current node that leads to next ancestor*/
-            cursor->nextAncestorPointerIdx[level] = cursor->entryIndex;
-            cursor->level = level;
-            
-            newEntryFromChild->ptr.child = NULL;
-            
-            return True;
-        }
-
-
-        /* If key already exists, update record and return success = True */
-        targetIdx = findChildIndex(node->entries, key, node->numKeys);
-        if (targetIdx != -1 && node->entries[targetIdx].key == key) {
-            node->entries[targetIdx].ptr.record = record;
-
-            cursor->currNode = node;
-            cursor->entryIndex = targetIdx;
-            cursor->isValid = True;
-                 
-            /*Set index of pointer in current node that leads to next ancestor*/
-            cursor->nextAncestorPointerIdx[level] = cursor->entryIndex;
-            cursor->level = level;
-            
-            newEntryFromChild->ptr.child = NULL;
-
-            return True;
-        }
-
-        /* if the leaf has space, insert key and record */
-        if (node->numKeys < FANOUT) {
-            int i;
-
-            /* Find first entry which newEntry is greater than or equal to
-             * key goes to the right of this index. */
-            const int targetIdx = findChildIndex(node->entries, key, node->numKeys);
-
-
-            /* Move all entries to the right of targetIdx one to the right*/
-            for (i = node->numKeys; i > targetIdx + 1; i--) {
-                /* move keys and pointers to the right */
-                node->entries[i] = node->entries[i - 1];
-            }
-
-            /* insert entry */
-            node->entries[targetIdx + 1].key = key;
-            node->entries[targetIdx + 1].ptr.record = record;
-            node->numKeys++;
-
-            newEntryFromChild->ptr.child = NULL;
-
-
-            /* Update cursor */
-            cursor->currNode = node;
-            cursor->entryIndex = targetIdx + 1;
-            cursor->isValid = True;
-            cursor->relation->numRecords++;
-            
-            /*Set index of pointer in current node that leads to next ancestor*/
-            cursor->nextAncestorPointerIdx[level] = cursor->entryIndex;
-            cursor->level = level;
-           
-            return True;
-        }
-        /* else split the leaf */
-        else {
-
-            /* Create an Array that can hold all entries. */
-            Entry allEntries[FANOUT + 1];
-            BtNode* newNode;
-            int i, j;
-            /* let the first node hold the floor of half of the FANOUT*/
-            int firstNodeSize = (FANOUT / 2);
-
-            /* index of first key that new Key is greater than or equal to  */
-            const int targetIdx = findChildIndex(node->entries, key, node->numKeys);
-
-            /* copy 0 to targetIdx of node's keys to allEntries, insert 
-             * newKeyFromChild, copy remaining targetIdx to MAXNUMKEYS - 1 
-             * keys to allEntries */
-            j = 0;
-            for (i = 0; i < FANOUT + 1; i++) {
-                if (i == (int) targetIdx + 1) {
-                    allEntries[i].key = key;
-                    allEntries[i].ptr.record = record;
-                } else {
-                    allEntries[i] = node->entries[j];
-                    j++;
-                }
-            }
-
-            /* overwrite current node with floor of first half of keys and 
-             * pointers. 
-             * TODO: Optimize later! Unnecessary copying over.
-             */
-            for (i = 0; i < firstNodeSize; i++) {
-                node->entries[i] = allEntries[i];
-            }
-            node->numKeys = firstNodeSize;
-
-            /* create a new leaf node to contain second half (including entry at 
-             * newEntryIdx) of split keys.
-             * copy them to new node */
-            newNode = createNewNode(True);
-            /* TODO: handle memory error better*/
-            assert(newNode);
-            j = 0;
-            for (i = firstNodeSize; i < FANOUT + 1; i++) {
-                newNode->entries[j] = allEntries[i];
-                j++;
-            }
-            newNode->numKeys = j;
-            newNode->ptr0 = NULL;
-
-            /*Set newEntryFromChild*/
-            newEntryFromChild->key = newNode->entries[0].key;
-            newEntryFromChild->ptr.child = newNode;
-
-
-            /* If this leaf is the root level, create new root, let it point to this 
-             * node and new Child entry. A new level has been created so move 
-             * all ancestor nodes and next ancestor ptr index to down one level.
-             */
-            if (relation->root == node) {
-                BtNode* newRootNode = createNewNode(False);
-                assert(newRootNode);
-
-                newRootNode->ptr0 = node;
-                newRootNode->numKeys = 1;
-                newRootNode->entries[0] = *newEntryFromChild;
-
-                relation->root = newRootNode;
-
-                newEntryFromChild->ptr.child = NULL;
-                                                
-                /* New level 0 ancestor, levels have increased*/
-                cursor->ancestors[0] = relation->root;    
-                cursor->level++;
-
-                if (targetIdx < firstNodeSize) {
-                    cursor->nextAncestorPointerIdx[0] = -1;
-                } else {
-                    cursor->nextAncestorPointerIdx[0] = 0;
-                }          
-                
-            }
-
-            /* If target index is less than firstNodeSize, then new key in 
-             * first node */
-            if (targetIdx + 1 < firstNodeSize) {
-                /* Update cursor */
-                cursor->currNode = node;
-                cursor->entryIndex = targetIdx + 1;
-                
-                /* nextAncestorIdx of parent might be new if*/
-                cursor->ancestors[cursor->level] = node;
-                cursor->nextAncestorPointerIdx[cursor->level] = cursor->entryIndex;
-            }                
-            /* Else, it is in the second node.*/
-            else {
-                /* Update cursor */
-                cursor->currNode = newNode;
-                cursor->entryIndex = targetIdx - (firstNodeSize - 1);
-                
-                /* nextAncestorIdx of parent might be new if*/
-                cursor->ancestors[cursor->level] = newNode;
-                cursor->nextAncestorPointerIdx[cursor->level] = cursor->entryIndex;
-            }
-
-            cursor->isValid = True;
-            cursor->relation->numRecords++;
-
-            return True;
-
+        allEntries[i] = node->entries[j];
+        j++;  
+    }
+    
+    /* if the new entry came before an entry in the first node, 
+     * then we need to update those entries in the first node.*/
+    if(tgtIdx < middle) {
+        for(i = tgtIdx; i < middle; i++) {
+            node->entries[i] = allEntries[i];   
         }
     }
-}
+    node->numKeys = middle;
+    
+    /* Create the new node. */
+    newNode = createNewNode(isLeaf,False,False);
+    assert(newNode);
 
+    /* Setting the LastLeaf boolean to newNode if needed */
+    if (node->LastLeaf == True) {
+      node->LastLeaf = False;
+      newNode->LastLeaf = True;
+    }
+    
+    /* Select appropriate idx to start copying. */
+    if(isLeaf) {
+        startIdx = middle;
+    } else {
+        /* We push up middle node, so don't copy it into snd node. */
+        startIdx = middle + 1;
+    }
+    
+    /*Copy entries to second node.*/
+    j = 0;
+    for (i = startIdx; i < FANOUT + 1; i++) {
+        newNode->entries[j] = allEntries[i];
+        j++;
+    }
+    newNode->numKeys = FANOUT + 1 - startIdx;
+    
+    newEntry = (Entry*) malloc(sizeof(Entry));
+    assert(newEntry != NULL);
+    
+    /* If this is a leaf, copy up first entry on second node. */
+    if(isLeaf) {
+        newEntry->key = allEntries[startIdx].key;
+        newEntry->ptr.child = newNode;
+    }
+    /* Else we are pushing up entry before second node. */
+    else {
+        newEntry->key = allEntries[startIdx - 1].key;
+        newEntry->ptr.child = newNode;
+	newNode->ptr0 = allEntries[startIdx - 1].ptr.child;
+    }
+
+    return newEntry; /* TODO */
+}
+  
+/* Inserting a new entry at a position given by the cursor.
+ * The cursor should point to the correct location: this function should only be called after goToKey
+ * If the key already exists in the relation, its record will be updated. */
+static void putEntry(Cursor_T cursor, int level, Entry * newEntry, size_t key) {
+  if (level==-1) {
+    /* the root has been split, and newEntry should be the only entry in the new root */
+    BtNode* currNode = createNewNode(False, False, False);
+    assert(currNode);
+
+    currNode->ptr0 = cursor->relation->root;
+    currNode->numKeys = 1;
+    currNode->entries[0] = *newEntry;
+
+    cursor->relation->root = currNode;
+    cursor->relation->depth ++;
+    cursor->relation->numRecords ++;
+    cursor->ancestors[0] = currNode;
+
+    /* we need to update the cursor for the original inserted key */
+    moveToKey(currNode, key, cursor, 0);
+    
+    return;
+  }
+
+  if (currNode(cursor)->isLeaf) { /* current node is a leaf node */
+    if (currNode(cursor)->entries[entryIndex(cursor)].key == newEntry->key) {
+      /* the key already exists in the cursor */
+      currNode(cursor)->entries[entryIndex(cursor)].ptr = newEntry->ptr;
+      return;
+    }
+    else {
+      /* the key does not exist and must be inserted */
+
+      if (currNode(cursor)->numKeys < FANOUT) {
+	const size_t tgtIdx = entryIndex(cursor);
+	
+	size_t i;
+	/* Move all entries to the right of tgtIdx one to the right*/
+	for (i=currNode(cursor)->numKeys; i > tgtIdx; i--) {
+	  currNode(cursor)->entries[i] = currNode(cursor)->entries[i-1];
+	}
+	currNode(cursor)->entries[tgtIdx] = *newEntry;
+	currNode(cursor)->numKeys++;
+	cursor->relation->numRecords++;
+	return;
+      }
+      else {
+	/* the leaf node must be split */
+	newEntry = splitnode(currNode(cursor), newEntry, True);
+	cursor->level--;
+	/* recursive call to insert the newEntry from splitnode a level above */
+	putEntry(cursor, level-1, newEntry, key);
+      }
+    }
+  }
+  else { /* current node is an intern node */
+    if (currNode(cursor)->numKeys < FANOUT) {
+      /* the current intern node has enough space to insert a new entry */
+      const size_t tgtIdx = cursor->ancestorsIdx[level] +1;
+      /* this is a correct index because there is enough space in the node */
+      
+      size_t i;
+      /* Move all entries to the right of tgtIdx one to the right*/
+      for (i=currNode(cursor)->numKeys; i > tgtIdx; i--) {
+	currNode(cursor)->entries[i] = currNode(cursor)->entries[i-1];
+      }
+      currNode(cursor)->entries[tgtIdx] = *newEntry;
+      currNode(cursor)->numKeys++;
+      cursor->relation->numRecords++; /* is that the good place to put it? */
+
+      /* update the cursor to make it point to the inserted key */
+      moveToKey(currNode(cursor), key, cursor, level);
+
+      return;
+    }
+    else {
+      /* the node must be split */
+      newEntry = splitnode(currNode(cursor), newEntry, False);
+      cursor->level--;
+      /* recursive call to insert the newEntry from splitnode a level above */
+      putEntry(cursor, level-1, newEntry, key);
+      
+    }
+  }
+}
 
 /* Algorithm from page 262 of Database Management Systems Second Edition. 
  * Delete key and record from the appropriate leaf in nodePtr. Use parentNode
@@ -863,62 +700,63 @@ static Bool deleteKeyRecord(BtNode* parentNode, BtNode* node, unsigned long key,
         Entry* const oldEntryFromChild, Cursor* cursor, Relation_T relation, 
         const int level){
     
-    Bool success;
-    int i;
+    /* Bool success; */
+    /* int i; */
     
-    /* Index of pointer to child tree containing key to be deleted */
-    int childTreePtrIdx;
+    /* /\* Index of pointer to child tree containing key to be deleted *\/ */
+    /* int childTreePtrIdx; */
     
-    assert(node != NULL);
-    assert(cursor != NULL);
-    /* Container to store new entry should never be NULL.*/
-    assert(oldEntryFromChild != NULL);
-    ASSERT_NODE_INVARIANT(node, relation);
+    /* assert(node != NULL); */
+    /* assert(cursor != NULL); */
+    /* /\* Container to store new entry should never be NULL.*\/ */
+    /* assert(oldEntryFromChild != NULL); */
+    /* ASSERT_NODE_INVARIANT(node, relation); */
         
-    if (node->isLeaf == False) {
-        BtNode* childNode;
+    /* if (node->isLeaf == False) { */
+    /*     BtNode* childNode; */
         
-        /* Get index of child node that contains. */
-        childTreePtrIdx = findChildIndex(node->entries, key, node->numKeys);
+    /*     /\* Get index of child node that contains. *\/ */
+    /*     childTreePtrIdx = findChildIndex(node->entries, key, node->numKeys); */
         
-        /* Get child node*/
-        if (childTreePtrIdx == -1) {
-            childNode = node->ptr0;
-        } else {
-            childNode = node->entries[childTreePtrIdx].ptr.child;
-        }
+    /*     /\* Get child node*\/ */
+    /*     if (childTreePtrIdx == -1) { */
+    /*         childNode = node->ptr0; */
+    /*     } else { */
+    /*         childNode = node->entries[childTreePtrIdx].ptr.child; */
+    /*     } */
                 
-        /* Recursively delete */
-        success = deleteKeyRecord(node, childNode, key, 
-                oldEntryFromChild, cursor, relation, level+1);
+    /*     /\* Recursively delete *\/ */
+    /*     success = deleteKeyRecord(node, childNode, key,  */
+    /*             oldEntryFromChild, cursor, relation, level+1); */
                 
-        /* if delete failed, return that delete failed */
-        if (success == False) {
-            return False;
-        }           
+    /*     /\* if delete failed, return that delete failed *\/ */
+    /*     if (success == False) { */
+    /*         return False; */
+    /*     }            */
         
-        /* else if successful and no merges, return success.*/
-        if (oldEntryFromChild->ptr.child == NULL) {
-            return success;
-        }
+    /*     /\* else if successful and no merges, return success.*\/ */
+    /*     if (oldEntryFromChild->ptr.child == NULL) { */
+    /*         return success; */
+    /*     } */
         
-        /* Handle case where entry / key has to be deleted in node because
-         * children were merged. */
-        return handleDeleteOfEntry(parentNode, node, 
-                oldEntryFromChild, cursor, relation, level);    
+    /*     /\* Handle case where entry / key has to be deleted in node because */
+    /*      * children were merged. *\/ */
+    /*     return handleDeleteOfEntry(parentNode, node,  */
+    /*             oldEntryFromChild, cursor, relation, level);     */
         
-    } 
-    /* Handle delete in child. */
-    else {
-        for (i = 0; i < node->numKeys; i++) {
-            if (node->entries[i].key == key) {
-                *oldEntryFromChild = node->entries[i];
-                return handleDeleteOfEntry(parentNode, node, oldEntryFromChild,
-                        cursor, relation, level);
-            }
-        }
-        return False;
-    }
+    /* }  */
+    /* /\* Handle delete in child. *\/ */
+    /* else { */
+    /*     for (i = 0; i < node->numKeys; i++) { */
+    /*         if (node->entries[i].key == key) { */
+    /*             *oldEntryFromChild = node->entries[i]; */
+    /*             return handleDeleteOfEntry(parentNode, node, oldEntryFromChild, */
+    /*                     cursor, relation, level); */
+    /*         } */
+    /*     } */
+    /*     return False; */
+    /* } */
+  return False;
 }
 
 
@@ -929,142 +767,143 @@ static Bool handleDeleteOfEntry(BtNode* parentNode, BtNode* node,
         Entry* const oldEntryFromChild, Cursor* cursor,
         Relation_T relation, const int level) {
 
-    int i, idx;
-    Bool found = False, wasMerged = False;
-    BtNode* leftSibling = NULL; 
-    BtNode* rightSibling = NULL;
+    /* int i, idx; */
+    /* Bool found = False, wasMerged = False; */
+    /* BtNode* leftSibling = NULL;  */
+    /* BtNode* rightSibling = NULL; */
 
-    assert(node != NULL);
-    assert(cursor != NULL);
-    assert(oldEntryFromChild != NULL);
+    /* assert(node != NULL); */
+    /* assert(cursor != NULL); */
+    /* assert(oldEntryFromChild != NULL); */
     
-    /* find the entry that matches oldEntry.*/
-    for (i = 0; i < node->numKeys; i++) {
-        /* if these entries match */
-        if ((oldEntryFromChild->key == node->entries[i].key) &&
-                (oldEntryFromChild->ptr.child == node->entries[i].ptr.child)) {
-            idx = i;
-            found = True;
-            break;
-        } 
-    }
+    /* /\* find the entry that matches oldEntry.*\/ */
+    /* for (i = 0; i < node->numKeys; i++) { */
+    /*     /\* if these entries match *\/ */
+    /*     if ((oldEntryFromChild->key == node->entries[i].key) && */
+    /*             (oldEntryFromChild->ptr.child == node->entries[i].ptr.child)) { */
+    /*         idx = i; */
+    /*         found = True; */
+    /*         break; */
+    /*     }  */
+    /* } */
     
-    assert(found == True);
+    /* assert(found == True); */
     
-    /* if found, delete the entry */
-    for(i = idx; i < node->numKeys - 1; i++) {
-        node->entries[i] = node->entries[i+1];
-    }
-    node->numKeys--;
+    /* /\* if found, delete the entry *\/ */
+    /* for(i = idx; i < node->numKeys - 1; i++) { */
+    /*     node->entries[i] = node->entries[i+1]; */
+    /* } */
+    /* node->numKeys--; */
     
-    /* MAKE SURE ENTRY IS NOT ROOT. Root is allowed to have less than FANOUT / 2
-     * entries. */
+    /* /\* MAKE SURE ENTRY IS NOT ROOT. Root is allowed to have less than FANOUT / 2 */
+    /*  * entries. *\/ */
     
-    /* If this is root. */
-    if(relation->root == node) {
-        /* if the root is now empty. and this is not a leaf. */
-        if (node->numKeys == 0 && node->isLeaf == False) {
-            /* Set the new root. */
-            relation->root = node->ptr0;
-            /* Free the old root. */
-            free(node);
-        }
-        /* Otherwise if this is a leaf, leave leaf node as root for insertion.*/
+    /* /\* If this is root. *\/ */
+    /* if(relation->root == node) { */
+    /*     /\* if the root is now empty. and this is not a leaf. *\/ */
+    /*     if (node->numKeys == 0 && node->isLeaf == False) { */
+    /*         /\* Set the new root. *\/ */
+    /*         relation->root = node->ptr0; */
+    /*         /\* Free the old root. *\/ */
+    /*         free(node); */
+    /*     } */
+    /*     /\* Otherwise if this is a leaf, leave leaf node as root for insertion.*\/ */
         
-        /* set oldEntryFromChild('s ptr) to NULL. */
-        oldEntryFromChild->ptr.child = NULL;
-        return True;  
-    }
+    /*     /\* set oldEntryFromChild('s ptr) to NULL. *\/ */
+    /*     oldEntryFromChild->ptr.child = NULL; */
+    /*     return True;   */
+    /* } */
     
     
-    /* if this not the root and the node had enough entries, set old entries 
-     * pointer to null to indicate that there is no node deleted at this level.
-     */
-    if (node->numKeys >= FANOUT/2) {
-        oldEntryFromChild->ptr.child = NULL;
-        return True;
-    }
+    /* /\* if this not the root and the node had enough entries, set old entries  */
+    /*  * pointer to null to indicate that there is no node deleted at this level. */
+    /*  *\/ */
+    /* if (node->numKeys >= FANOUT/2) { */
+    /*     oldEntryFromChild->ptr.child = NULL; */
+    /*     return True; */
+    /* } */
     
-    /* Else redistribute or merge. */
+    /* /\* Else redistribute or merge. *\/ */
     
-    found = False;
-    for(i=0; i < parentNode->numKeys; i++) {
-        if(parentNode->entries[i].ptr.child == node) {
-            found = True;
-            idx = i;
-            break;
-        }
-    }
+    /* found = False; */
+    /* for(i=0; i < parentNode->numKeys; i++) { */
+    /*     if(parentNode->entries[i].ptr.child == node) { */
+    /*         found = True; */
+    /*         idx = i; */
+    /*         break; */
+    /*     } */
+    /* } */
     
-    if (parentNode->ptr0 != node) {
-        assert(found == True);
-    }
+    /* if (parentNode->ptr0 != node) { */
+    /*     assert(found == True); */
+    /* } */
     
-    /* First get sibling(s). Non-root nodes must have at least one sibling. */
-    /* if node is leftmost or rightmost child, only one sibling */
-    if(parentNode->ptr0 == node) {
-        rightSibling = parentNode->entries[0].ptr.child;
-    } 
-    else if (parentNode->entries[parentNode->numKeys - 1].ptr.child == node) {
-        leftSibling = parentNode->entries[parentNode->numKeys - 2].ptr.child;
-    } 
-    /* otherwise, one or two siblings*/
-    else {
+    /* /\* First get sibling(s). Non-root nodes must have at least one sibling. *\/ */
+    /* /\* if node is leftmost or rightmost child, only one sibling *\/ */
+    /* if(parentNode->ptr0 == node) { */
+    /*     rightSibling = parentNode->entries[0].ptr.child; */
+    /* }  */
+    /* else if (parentNode->entries[parentNode->numKeys - 1].ptr.child == node) { */
+    /*     leftSibling = parentNode->entries[parentNode->numKeys - 2].ptr.child; */
+    /* }  */
+    /* /\* otherwise, one or two siblings*\/ */
+    /* else { */
         
-        /* Get left sibling. */
-        if(idx == 0){
-            leftSibling = parentNode->ptr0;
-        } else {
-            leftSibling = parentNode->entries[idx - 1].ptr.child;
-        }
+    /*     /\* Get left sibling. *\/ */
+    /*     if(idx == 0){ */
+    /*         leftSibling = parentNode->ptr0; */
+    /*     } else { */
+    /*         leftSibling = parentNode->entries[idx - 1].ptr.child; */
+    /*     } */
         
-        /* Get right sibling. */
-        if(idx + 1 < parentNode->numKeys) {
-            rightSibling = parentNode->entries[idx + 1].ptr.child;
-        }
-    }
+    /*     /\* Get right sibling. *\/ */
+    /*     if(idx + 1 < parentNode->numKeys) { */
+    /*         rightSibling = parentNode->entries[idx + 1].ptr.child; */
+    /*     } */
+    /* } */
     
-    /* There must be a sibling as this is not the root. */
-    assert(leftSibling != NULL || rightSibling != NULL);
+    /* /\* There must be a sibling as this is not the root. *\/ */
+    /* assert(leftSibling != NULL || rightSibling != NULL); */
     
-    /* Now attempt redistribute or merge using node and smallest sibling. We use
-     * the smallest sibling as this increases the chance of redistributions 
-     * which is more favorable as redistributions do not propagate*/
+    /* /\* Now attempt redistribute or merge using node and smallest sibling. We use */
+    /*  * the smallest sibling as this increases the chance of redistributions  */
+    /*  * which is more favorable as redistributions do not propagate*\/ */
     
-    if(rightSibling == NULL) {
-        rightSibling = node;
-    } else if (leftSibling == NULL) {
-        leftSibling = node;
-    } else if (leftSibling->numKeys <= rightSibling->numKeys) {
-        rightSibling = node;
-    } else {
-        leftSibling = node;
-    }
+    /* if(rightSibling == NULL) { */
+    /*     rightSibling = node; */
+    /* } else if (leftSibling == NULL) { */
+    /*     leftSibling = node; */
+    /* } else if (leftSibling->numKeys <= rightSibling->numKeys) { */
+    /*     rightSibling = node; */
+    /* } else { */
+    /*     leftSibling = node; */
+    /* } */
     
-    /* Find splitting parent entry. */
-    found = False;
-    for(idx = 0; idx < parentNode->numKeys; idx++) {
-        if(parentNode->entries[idx].ptr.child == rightSibling) {
-            found = True;
-            break;
-        }
-    }
+    /* /\* Find splitting parent entry. *\/ */
+    /* found = False; */
+    /* for(idx = 0; idx < parentNode->numKeys; idx++) { */
+    /*     if(parentNode->entries[idx].ptr.child == rightSibling) { */
+    /*         found = True; */
+    /*         break; */
+    /*     } */
+    /* } */
     
-    assert(found == True);
+    /* assert(found == True); */
     
-    redistributeOrMerge(leftSibling, rightSibling, &(parentNode->entries[idx]), 
-                        leftSibling->isLeaf, &wasMerged);
+    /* redistributeOrMerge(leftSibling, rightSibling, &(parentNode->entries[idx]),  */
+    /*                     leftSibling->isLeaf, &wasMerged); */
     
-    /* If nodes weren't merged, set oldEntryFromChild to false, return True*/
-    if(wasMerged == False){
-        oldEntryFromChild->ptr.child = NULL;
-        return True;
-    }
-    /* Else splitting entry has to be deleted in parent. And right node
-     * should be freed as its entries have been merged into left node. */
-    *oldEntryFromChild = parentNode->entries[idx];
-    free(rightSibling);
-    return True;
+    /* /\* If nodes weren't merged, set oldEntryFromChild to false, return True*\/ */
+    /* if(wasMerged == False){ */
+    /*     oldEntryFromChild->ptr.child = NULL; */
+    /*     return True; */
+    /* } */
+    /* /\* Else splitting entry has to be deleted in parent. And right node */
+    /*  * should be freed as its entries have been merged into left node. *\/ */
+    /* *oldEntryFromChild = parentNode->entries[idx]; */
+    /* free(rightSibling); */
+    /* return True; */
+  return False;
 }
 
 
@@ -1081,147 +920,147 @@ static Bool handleDeleteOfEntry(BtNode* parentNode, BtNode* node,
  */
 static void redistributeOrMerge(BtNode* leftNode, BtNode* rightNode,
         Entry* const parentEntry, Bool isLeaf,  Bool* wasMerged) {
-    int totalKeys = leftNode->numKeys + rightNode->numKeys;
-    int i;
+    /* int totalKeys = leftNode->numKeys + rightNode->numKeys; */
+    /* int i; */
     
-    assert(leftNode != NULL);
-    assert(rightNode != NULL);
-    /* Assert there are enough keys for redistribution or a merge.*/
-    assert(totalKeys >= FANOUT / 2);
+    /* assert(leftNode != NULL); */
+    /* assert(rightNode != NULL); */
+    /* /\* Assert there are enough keys for redistribution or a merge.*\/ */
+    /* assert(totalKeys >= FANOUT / 2); */
     
-    /* Algorithm for redistributing or merging in non-Leaf. */
-    if (isLeaf == False) {
-        /* If the total number of keys is greater than FANOUT, we can and 
-         * should redistribute. */
-        if(totalKeys >= FANOUT) {
-            /* if the left node has less keys, redistribute from right to left. */
-            if (leftNode->numKeys < rightNode->numKeys) {
-                /* while the left node is smaller than the right node, redistribute*/
-                while(leftNode->numKeys < rightNode->numKeys){
-                    /* copy parentEntry key into new space on left node*/
-                    leftNode->entries[leftNode->numKeys].key = parentEntry->key;
-                    /* copy right node's key into parentEntry key*/
-                    parentEntry->key = rightNode->entries[0].key;
+    /* /\* Algorithm for redistributing or merging in non-Leaf. *\/ */
+    /* if (isLeaf == False) { */
+    /*     /\* If the total number of keys is greater than FANOUT, we can and  */
+    /*      * should redistribute. *\/ */
+    /*     if(totalKeys >= FANOUT) { */
+    /*         /\* if the left node has less keys, redistribute from right to left. *\/ */
+    /*         if (leftNode->numKeys < rightNode->numKeys) { */
+    /*             /\* while the left node is smaller than the right node, redistribute*\/ */
+    /*             while(leftNode->numKeys < rightNode->numKeys){ */
+    /*                 /\* copy parentEntry key into new space on left node*\/ */
+    /*                 leftNode->entries[leftNode->numKeys].key = parentEntry->key; */
+    /*                 /\* copy right node's key into parentEntry key*\/ */
+    /*                 parentEntry->key = rightNode->entries[0].key; */
 
-                    /* Move Pointers appropriately. */
-                    leftNode->entries[leftNode->numKeys].ptr.child = rightNode->ptr0;
-                    rightNode->ptr0 = rightNode->entries[0].ptr.child;
+    /*                 /\* Move Pointers appropriately. *\/ */
+    /*                 leftNode->entries[leftNode->numKeys].ptr.child = rightNode->ptr0; */
+    /*                 rightNode->ptr0 = rightNode->entries[0].ptr.child; */
                     
-                    /* Delete first entry*/
-                    for (i = 1; i < rightNode->numKeys; i++) {
-                        rightNode->entries[i-1] = rightNode->entries[i];
-                    }
-                    leftNode->numKeys++;
-                    rightNode->numKeys--;
-                }
-            }
-            /* else right node has less keys, so redistribute from left to right. */
-            else {
-                /* while the right node is smaller than the left node, redistribute*/
-                while(rightNode->numKeys < leftNode->numKeys){
-                    /* make space for a new entry on the right node */
-                    for (i = rightNode->numKeys; i > 0; i--) {
-                        rightNode->entries[i] = rightNode->entries[i-1];
-                    }
+    /*                 /\* Delete first entry*\/ */
+    /*                 for (i = 1; i < rightNode->numKeys; i++) { */
+    /*                     rightNode->entries[i-1] = rightNode->entries[i]; */
+    /*                 } */
+    /*                 leftNode->numKeys++; */
+    /*                 rightNode->numKeys--; */
+    /*             } */
+    /*         } */
+    /*         /\* else right node has less keys, so redistribute from left to right. *\/ */
+    /*         else { */
+    /*             /\* while the right node is smaller than the left node, redistribute*\/ */
+    /*             while(rightNode->numKeys < leftNode->numKeys){ */
+    /*                 /\* make space for a new entry on the right node *\/ */
+    /*                 for (i = rightNode->numKeys; i > 0; i--) { */
+    /*                     rightNode->entries[i] = rightNode->entries[i-1]; */
+    /*                 } */
 
-                    /* copy parentEntry key into new space on right node*/
-                    rightNode->entries[0].key = parentEntry->key;
-                    /* copy left node's last key into parentEntry key*/
-                    parentEntry->key = leftNode->entries[leftNode->numKeys-1].key;
+    /*                 /\* copy parentEntry key into new space on right node*\/ */
+    /*                 rightNode->entries[0].key = parentEntry->key; */
+    /*                 /\* copy left node's last key into parentEntry key*\/ */
+    /*                 parentEntry->key = leftNode->entries[leftNode->numKeys-1].key; */
                     
-                    /* Move Pointers appropriately. */
-                    rightNode->entries[0].ptr.child = rightNode->ptr0;
-                    rightNode->ptr0 = leftNode->entries[leftNode->numKeys-1].ptr.child;
+    /*                 /\* Move Pointers appropriately. *\/ */
+    /*                 rightNode->entries[0].ptr.child = rightNode->ptr0; */
+    /*                 rightNode->ptr0 = leftNode->entries[leftNode->numKeys-1].ptr.child; */
                     
 
-                    leftNode->numKeys--;
-                    rightNode->numKeys++;
-                }
-            }
+    /*                 leftNode->numKeys--; */
+    /*                 rightNode->numKeys++; */
+    /*             } */
+    /*         } */
 
-            *wasMerged = False;
-        }
-        /* else if not enough total keys for two nodes, merge both nodes. */
-        else {
-            /* First copy parent splitting key and left most pointer in right node
-             * as new entry in left node. */
-            leftNode->entries[leftNode->numKeys].key = parentEntry->key;
-            leftNode->entries[leftNode->numKeys].ptr.child = rightNode->ptr0;
-            leftNode->numKeys++;
+    /*         *wasMerged = False; */
+    /*     } */
+    /*     /\* else if not enough total keys for two nodes, merge both nodes. *\/ */
+    /*     else { */
+    /*         /\* First copy parent splitting key and left most pointer in right node */
+    /*          * as new entry in left node. *\/ */
+    /*         leftNode->entries[leftNode->numKeys].key = parentEntry->key; */
+    /*         leftNode->entries[leftNode->numKeys].ptr.child = rightNode->ptr0; */
+    /*         leftNode->numKeys++; */
 
-            /* Move all entries from right node and add them to left node. */
-            for(i = 0; i < rightNode->numKeys; i++) {
-                leftNode->entries[leftNode->numKeys] = rightNode->entries[i];
-                leftNode->numKeys++;
-            }
+    /*         /\* Move all entries from right node and add them to left node. *\/ */
+    /*         for(i = 0; i < rightNode->numKeys; i++) { */
+    /*             leftNode->entries[leftNode->numKeys] = rightNode->entries[i]; */
+    /*             leftNode->numKeys++; */
+    /*         } */
 
-            *wasMerged = True;
-        }
-    }
-    /* Algorithm for redistributing or merging in leaf. */
-    else {
-        /* If the total number of keys is greater than FANOUT, we can and 
-         * should redistribute. */
-        if(totalKeys >= FANOUT) {
-            /* if the left node has less keys, redistribute from right to left. */
-            if (leftNode->numKeys < rightNode->numKeys) {
-                /* while the left node is smaller than the right node, redistribute*/
-                while(leftNode->numKeys < rightNode->numKeys){
-                    /* copy entry from the right node to the left node. */
-                    leftNode->entries[leftNode->numKeys] = rightNode->entries[0];
+    /*         *wasMerged = True; */
+    /*     } */
+    /* } */
+    /* /\* Algorithm for redistributing or merging in leaf. *\/ */
+    /* else { */
+    /*     /\* If the total number of keys is greater than FANOUT, we can and  */
+    /*      * should redistribute. *\/ */
+    /*     if(totalKeys >= FANOUT) { */
+    /*         /\* if the left node has less keys, redistribute from right to left. *\/ */
+    /*         if (leftNode->numKeys < rightNode->numKeys) { */
+    /*             /\* while the left node is smaller than the right node, redistribute*\/ */
+    /*             while(leftNode->numKeys < rightNode->numKeys){ */
+    /*                 /\* copy entry from the right node to the left node. *\/ */
+    /*                 leftNode->entries[leftNode->numKeys] = rightNode->entries[0]; */
                    
-                    /* Delete first entry*/
-                    for (i = 1; i < rightNode->numKeys; i++) {
-                        rightNode->entries[i-1] = rightNode->entries[i];
-                    }
+    /*                 /\* Delete first entry*\/ */
+    /*                 for (i = 1; i < rightNode->numKeys; i++) { */
+    /*                     rightNode->entries[i-1] = rightNode->entries[i]; */
+    /*                 } */
                     
-                    /* Set new splitting key in parent. */
-                    parentEntry->key = rightNode->entries[0].key;
+    /*                 /\* Set new splitting key in parent. *\/ */
+    /*                 parentEntry->key = rightNode->entries[0].key; */
                     
-                    leftNode->numKeys++;
-                    rightNode->numKeys--;
-                }
-            }
-            /* else right node has less keys, so redistribute from left to right. */
-            else {
-                /* while the right node is smaller than the left node, redistribute*/
-                while(rightNode->numKeys < leftNode->numKeys){
-                    /* make space for a new entry on the right node */
-                    for (i = rightNode->numKeys; i > 0; i--) {
-                        rightNode->entries[i] = rightNode->entries[i-1];
-                    }
+    /*                 leftNode->numKeys++; */
+    /*                 rightNode->numKeys--; */
+    /*             } */
+    /*         } */
+    /*         /\* else right node has less keys, so redistribute from left to right. *\/ */
+    /*         else { */
+    /*             /\* while the right node is smaller than the left node, redistribute*\/ */
+    /*             while(rightNode->numKeys < leftNode->numKeys){ */
+    /*                 /\* make space for a new entry on the right node *\/ */
+    /*                 for (i = rightNode->numKeys; i > 0; i--) { */
+    /*                     rightNode->entries[i] = rightNode->entries[i-1]; */
+    /*                 } */
                     
-                    /* copy entry from the left node to the right node. */
-                    rightNode->entries[0] = leftNode->entries[leftNode->numKeys-1];
+    /*                 /\* copy entry from the left node to the right node. *\/ */
+    /*                 rightNode->entries[0] = leftNode->entries[leftNode->numKeys-1]; */
                     
-                    /* set new splitting key in parent. */
-                    parentEntry->key = rightNode->entries[0].key;
+    /*                 /\* set new splitting key in parent. *\/ */
+    /*                 parentEntry->key = rightNode->entries[0].key; */
 
-                    leftNode->numKeys--;
-                    rightNode->numKeys++;
-                }
-            }
+    /*                 leftNode->numKeys--; */
+    /*                 rightNode->numKeys++; */
+    /*             } */
+    /*         } */
 
-            *wasMerged = False;
-        }
-        /* else if not enough total keys for two nodes, merge both nodes. */
-        else {
+    /*         *wasMerged = False; */
+    /*     } */
+    /*     /\* else if not enough total keys for two nodes, merge both nodes. *\/ */
+    /*     else { */
 
-            /* Move all entries from right node and add them to left node. */
-            for(i = 0; i < rightNode->numKeys; i++) {
-                leftNode->entries[leftNode->numKeys] = rightNode->entries[i];
-                leftNode->numKeys++;
-            }
+    /*         /\* Move all entries from right node and add them to left node. *\/ */
+    /*         for(i = 0; i < rightNode->numKeys; i++) { */
+    /*             leftNode->entries[leftNode->numKeys] = rightNode->entries[i]; */
+    /*             leftNode->numKeys++; */
+    /*         } */
 
-            *wasMerged = True;
-        }
-    }
-    
+    /*         *wasMerged = True; */
+    /*     } */
+    /* } */
+  return;    
 }
 
 
 
-/* Given an array of entries, find the index of the first entry whose key is
+/* Given an array of entries, find the index of the last entry whose key is
  * less than or equal to the search key. */
 static int findChildIndex(const Entry* entries, unsigned long key, int length) {
     int i = 0;
@@ -1235,134 +1074,138 @@ static int findChildIndex(const Entry* entries, unsigned long key, int length) {
     }
     /* else see if key falls in between any two keys, return index of first key*/
     for (i = 0; i <= length - 2; i++) {
-        if (key >= entries[i].key && key < entries[i + 1].key)
+      if (key >= entries[i].key && key < entries[i + 1].key) {
             return i;
+      }
     }
     /* if key greater or equal to last element, return index of last element*/
     return length - 1;
 }
 
-/* move cursor to key in node. On finding key's record, return True and update cursor. 
- * If relation empty or key not in B+-tree, return False */
-static Bool moveToRecord(BtNode* node, unsigned long key, Cursor* cursor, 
-        const int level, int *pRes) {
-    cursor->ancestors[level] = node;
-   
-    if (node->isLeaf) {
-        int i;
-        
-        if (node->numKeys == 0) {
-            /* Should never have a non-root leaf node with zero numkeys*/
-            assert(level == 0);
-            cursor->isValid = False;
-            return False;
-        }
-        
-        i = findChildIndex(node->entries, key, node->numKeys);
-        cursor->currNode = node;
-        cursor->isValid = True;
-        cursor->level = level;
+/* Given an array of entries, find the index of the first entry whose key is
+ * greater than or equal to the search key. */
+static int findRecordIndex(const Entry* entries, unsigned long key, int length) {
+  int i = 0;
+  assert(entries != NULL);
+  assert(length >= 0);
 
-        
-        if(i == -1) {
-            cursor->entryIndex = 0;
-            cursor->nextAncestorPointerIdx[level] = cursor->entryIndex;
-            /* key at cursor loc greater than desired key*/
-            *pRes = 1;
-        }
-        else if (node->entries[i].key == key) {
-            cursor->entryIndex = i;
-            cursor->nextAncestorPointerIdx[level] = cursor->entryIndex;
-            /* key at cursor loc is same as desired key*/
-            *pRes = 0;
-        }  
-        else {
-            cursor->entryIndex = i;
-            cursor->nextAncestorPointerIdx[level] = cursor->entryIndex;
-            /* key at cursor loc less than desired key*/
-            *pRes = -1;
-        }   
-        
-        if (*pRes == 0) {
-            return True;
-        }
-        return False;
-        
-    } else {
-        int i;
-        BtNode* child;
-        
-        i = findChildIndex(node->entries, key, node->numKeys);
-        cursor->nextAncestorPointerIdx[level] = i;
-        
-        if (i == -1) {
-            child = node->ptr0;
-        } else {
-            child = node->entries[i].ptr.child;
-        }
-        
-        return moveToRecord(child, key, cursor, level + 1, pRes);
+  if (length == 0) {
+    return 0;
+  }
+
+  for (i = 0; i <= length - 1; i++) {
+    if (key <= entries[i].key) {
+      return i;
     }
+  }
+
+  /* if the key is strictly greater than any key in the node */
+  return length;
+}
+
+
+/* move cursor to key in node. On finding key's record, return True and update cursor.
+ * The function assumes that node is a parent of the key
+ * If relation empty or key not in B+-tree, return False */
+static void moveToKey(BtNode* node, unsigned long key, Cursor* cursor, const int level) {
+  cursor->ancestors[level] = node;
+  
+  if (node->isLeaf) {
+    cursor->level = level;
+    cursor->ancestorsIdx[level] = findRecordIndex(node->entries, key, node->numKeys);
+    return;
+    
+  } else { /* intern node */
+    int i;
+    BtNode* child;
+    
+    i = findChildIndex(node->entries, key, node->numKeys);
+    cursor->ancestorsIdx[level] = i;
+    
+    if (i == -1) {
+      child = node->ptr0;
+    } else {
+      child = node->entries[i].ptr.child;
+    }
+    
+    moveToKey(child, key, cursor, level + 1);
+    return;
+  }
 }
 
 /* Move to the first record in the B-tree*/
-static Bool moveToFirstRecord(BtNode* node, Cursor* cursor, int level) {
-    assert(node != NULL);
-    assert(cursor != NULL);
-    assert(level >= 0);
-    
-    /* Track ancestors as you go to first node*/
-    cursor->ancestors[level] = node;
-    cursor->nextAncestorPointerIdx[level] = -1;
-            
-    if (node->isLeaf) {
-        if (node->numKeys == 0) {
-            return False;
-        }
-        
-        cursor->currNode = node;
-        cursor->entryIndex = 0;
-        cursor->nextAncestorPointerIdx[level] = 0;
-        cursor->level = level;
-        
-        return True;
-    }
-    
-    return moveToFirstRecord(node->ptr0, cursor, level+1);
+static void moveToFirst(BtNode* node, Cursor* cursor, int level) {
+  assert(node != NULL);
+  assert(cursor != NULL);
+  assert(level >= 0);
+  
+  /* Track ancestors as you go to first node*/
+  cursor->ancestors[level] = node;
+  cursor->level = level;
+  
+  if (node->isLeaf) {
+    cursor->ancestorsIdx[level] = 0;
+    return;
+  }
+
+  /* Otherwise intern node, we need to keep going down */
+  cursor->ancestorsIdx[level] = -1;
+  moveToFirst(node->ptr0, cursor, level+1);
+  return;
 }
+
+static void moveToLast(BtNode* node, Cursor* cursor, int level) {
+  assert(node != NULL);
+  assert(cursor != NULL);
+  assert(level >= 0);
+
+  cursor->ancestors[level] = node;
+  cursor->level = level;
+  
+  if (node->isLeaf) {
+    cursor->ancestorsIdx[level] = node->numKeys;
+    return;
+  }
+
+  /* Otherwise intern node, we need to keep going down */
+  cursor->ancestorsIdx[level] = node->numKeys-1;
+  moveToFirst(node->entries[node->numKeys-1].ptr.child, cursor, level+1);
+  return;
+}  
 
 static void handleDeleteBtree(BtNode* node, void (* freeRecord)(void *)) {
-    int i;
+    /* int i; */
     
-    /* Part of base case. In leaf node, free all records with 
-     * freeRecord function, if any. */
-    if (node->isLeaf) {
-        if (freeRecord == NULL){
-            return;
-        }
+    /* /\* Part of base case. In leaf node, free all records with  */
+    /*  * freeRecord function, if any. *\/ */
+    /* if (node->isLeaf) { */
+    /*     if (freeRecord == NULL){ */
+    /*         return; */
+    /*     } */
         
-        for (i = 0; i < node->numKeys; i++) {
-            freeRecord((void *)node->entries[i].ptr.record);
-        }
+    /*     for (i = 0; i < node->numKeys; i++) { */
+    /*         freeRecord((void *)node->entries[i].ptr.record); */
+    /*     } */
         
-        return;
-    }
+    /*     return; */
+    /* } */
     
-    /* Recursively delete every child subtree. If the child is a leaf, after 
-     * recursively deleting every child subtree, free the node. */
-    handleDeleteBtree(node->ptr0, freeRecord);
-    if (node->ptr0->isLeaf) {
-        free(node->ptr0);
-    }
-    for(i = 0; i < node->numKeys; i++) {
-        handleDeleteBtree(node->entries[i].ptr.child, freeRecord);
-        if (node->entries[i].ptr.child->isLeaf) {
-            free(node->entries[i].ptr.child);
-        }
-    }
+    /* /\* Recursively delete every child subtree. If the child is a leaf, after  */
+    /*  * recursively deleting every child subtree, free the node. *\/ */
+    /* handleDeleteBtree(node->ptr0, freeRecord); */
+    /* if (node->ptr0->isLeaf) { */
+    /*     free(node->ptr0); */
+    /* } */
+    /* for(i = 0; i < node->numKeys; i++) { */
+    /*     handleDeleteBtree(node->entries[i].ptr.child, freeRecord); */
+    /*     if (node->entries[i].ptr.child->isLeaf) { */
+    /*         free(node->entries[i].ptr.child); */
+    /*     } */
+    /* } */
+  return;
 }
 
-/* Chck node size invariants */
+/* Check node size invariants */
 static void ASSERT_NODE_INVARIANT(BtNode* node, Relation_T relation) {
     
     /* If not root, must have at least fanout / 2 keys*/
@@ -1393,7 +1236,7 @@ static void printTree(BtNode* node, int level) {
     int i;
     
     if(node->isLeaf) {
-        fprintf(stderr, "Level: %d ", level);
+        fprintf(stderr, "Leaf Level: %d) ", level);
         for(i = 0; i < node->numKeys; i++) {
             fprintf(stderr, " %lu", node->entries[i].key);
         }
@@ -1401,7 +1244,7 @@ static void printTree(BtNode* node, int level) {
         return;
     }
     
-    fprintf(stderr, "Level: %d ", level);
+    fprintf(stderr, "Intern Level: %d) ", level);
     for(i = 0; i < node->numKeys; i++) {
         fprintf(stderr, " %lu", node->entries[i].key);
     }
@@ -1411,4 +1254,13 @@ static void printTree(BtNode* node, int level) {
     for(i = 0; i < node->numKeys; i++) {
         printTree(node->entries[i].ptr.child, level+1);
     }
+}
+
+static void printCursor(Cursor_T cursor) {
+  int i;
+  printf("Cursor: ");
+  for (i=0; i <= cursor->level; i++) {
+    printf("%d ", cursor->ancestorsIdx[i]);
+  }
+  printf("\n");
 }
