verif/btrees_sep.v
@@ -12,6 +12,7 @@ Require Import VST.floyd.reassoc_seq.
 Require Import VST.floyd.field_at_wand.
 Require Import FunInd.
 Require Import btrees.
+Require Import index.
 
 (**
     REPRESENTATIONS IN SEPARATION LOGIC
@@ -27,10 +28,10 @@ Definition value_rep (v:V) (p:val):= (* this should change if we change the type
   data_at Tsh tint (Vint (Int.repr v)) p.
 
 Definition isLeaf {X:Type} (n:node X) : bool :=
-  match n with btnode ptr0 le b w => b end.
+  match n with btnode ptr0 le b First Last w => b end.
 
 Definition getval (n:node val): val :=
-  match n with btnode _ _ _ x => x end.
+  match n with btnode _ _ _ _ _ x => x end.
 
 Fixpoint le_to_list (le:listentry val) : list (val * (val + val)) :=
   match le with
@@ -47,18 +48,20 @@ Definition le_to_list_complete (le:listentry val):=
                         
 Fixpoint entry_rep (e:entry val):=
   match e with
-  | keychild _ n => match n with btnode _ _ _ x => btnode_rep n x end
+  | keychild _ n => match n with btnode _ _ _ _ _ x => btnode_rep n x end
   | keyval _ v x => value_rep v x
   end
 with btnode_rep (n:node val) (p:val):mpred :=
-  match n with btnode ptr0 le b x =>
+  match n with btnode ptr0 le b First Last x =>
   !!(x=p) &&
   malloc_token Tsh tbtnode p *
   field_at Tsh tbtnode (DOT _numKeys) (Vint(Int.repr (Z.of_nat (numKeys n)))) p *
   field_at Tsh tbtnode (DOT _isLeaf) (Val.of_bool b) p *
+  field_at Tsh tbtnode (DOT _FirstLeaf) (Val.of_bool First) p *
+  field_at Tsh tbtnode (DOT _LastLeaf) (Val.of_bool Last) p *
   match ptr0 with
   | None => field_at Tsh tbtnode (DOT _ptr0) nullval p
-  | Some n' => match n' with btnode _ _ _ p' => field_at Tsh tbtnode (DOT _ptr0) p' p * btnode_rep n' p' end
+  | Some n' => match n' with btnode _ _ _ _ _ p' => field_at Tsh tbtnode (DOT _ptr0) p' p * btnode_rep n' p' end
   end *
   field_at Tsh tbtnode (DOT _entries) (le_to_list_complete le) p *
   le_iter_sepcon le
@@ -69,9 +72,6 @@ with le_iter_sepcon (le:listentry val):mpred :=
   | cons e le' => entry_rep e * le_iter_sepcon le'
   end.
 
-Definition get_val (n:node val) : val :=
-  match n with btnode _ _ _ x => x end.
-
 Lemma btnode_rep_local_prop: forall n p,
     btnode_rep n p |-- !!(isptr p).
 Proof.
@@ -79,7 +79,7 @@ Proof.
 Qed.
 
 Lemma btnode_rep_local_prop2: forall n p,
-    btnode_rep n p |-- !!(p = get_val n).
+    btnode_rep n p |-- !!(p = getval n).
 Proof.
   intros. destruct n. unfold btnode_rep. Intros. subst. entailer!.
 Qed.
@@ -97,24 +97,25 @@ Hint Resolve btnode_valid_pointer: valid_pointer.
 
 Definition relation_rep (r:relation val) (p:val):mpred :=
   match r with
-  | (n,c,x) => !!(x=p) &&
+  | (n,c,d,x) => !!(x=p) &&
     EX p':val,
           field_at Tsh trelation (DOT _root) p' p *
           btnode_rep n p' *
-          field_at Tsh trelation (DOT _numRecords) (Vlong(Int64.repr(Z.of_nat c))) p * (* long?int? *)
+          field_at Tsh trelation (DOT _numRecords) (Vint(Int.repr(Z.of_nat c))) p *
+          field_at Tsh trelation (DOT _depth) (Vint (Int.repr (Z.of_nat d))) p *
           malloc_token Tsh trelation p
   end.
 
 Lemma relation_rep_local_prop: forall r p,
     relation_rep r p |-- !!(isptr p).
 Proof. 
-  intros. destruct r. unfold relation_rep. destruct p0. Intros p'. entailer!.
+  intros. destruct r. unfold relation_rep. destruct p0. destruct p0. Intros p'. entailer!.
 Qed.
 
 Lemma relation_rep_local_prop2: forall r p,
     relation_rep r p |-- !!(p = snd r).
 Proof. 
-  intros. destruct r. unfold relation_rep. destruct p0. Intros p'. entailer!.
+  intros. destruct r. unfold relation_rep. destruct p0. destruct p0. Intros p'. entailer!.
 Qed.
 
 Hint Resolve relation_rep_local_prop: saturate_local.
@@ -123,7 +124,7 @@ Hint Resolve relation_rep_local_prop2: saturate_local.
 Lemma relation_rep_valid_pointer: forall r p,
     relation_rep r p |-- valid_pointer p.
 Proof.
-  intros. destruct r. unfold relation_rep. destruct p0. Intros p'. entailer!.
+  intros. destruct r. unfold relation_rep. destruct p0. destruct p0. Intros p'. entailer!.
 Qed.
 
 Hint Resolve relation_rep_valid_pointer: valid_pointer.
@@ -131,19 +132,13 @@ Hint Resolve relation_rep_valid_pointer: valid_pointer.
 Definition getCurrVal (c:cursor val): val :=
   match c with
   | [] => nullval
-  | (n,_)::_ => match n with btnode _ _ _ x => x end
-  end.
-
-Definition getEntryIndex {X:Type} (c:cursor X) : index :=
-  match c with
-  | (n,i)::_ => i
-  | [] => ip (0%nat)
+  | (n,_)::_ => getval n
   end.
 
 Fixpoint cursor_valid_bool {X:Type} (c:cursor X): bool :=
   match c with
   | [] => true
-  | (b,i)::c' => match b with btnode ptr0 le _ x => (index_leb_nat i (numKeys_le le -1)) && cursor_valid_bool c' end
+  | (b,i)::c' => match b with btnode ptr0 le _ _ _ x => (index_leb_nat i (numKeys_le le -1)) && cursor_valid_bool c' end
   end.                          (* might be incomplete *)
 
 Definition rep_index (i:index):=
@@ -155,12 +150,9 @@ Definition rep_index (i:index):=
 Definition cursor_rep (c:cursor val) (r:relation val) (p:val):mpred :=
   EX anc_end:list val, EX idx_end:list val,
   malloc_token Tsh tcursor p *
-  field_at Tsh tcursor (DOT _currNode) (getCurrVal c) p *
   match r with (n,c,x) => field_at Tsh tcursor (DOT _relation) x p end *
-  field_at Tsh tcursor (DOT _entryIndex) (rep_index(getEntryIndex c)) p *
-  field_at Tsh tcursor (DOT _isValid) (Val.of_bool (cursor_valid_bool c)) p *
   field_at Tsh tcursor (DOT _level) (Vint(Int.repr(Zlength c))) p *
-  field_at Tsh tcursor (DOT _nextAncestorPointerIdx) ((map (fun x => (rep_index (snd x)))  c) ++ idx_end) p * (* or its reverse? *)
+  field_at Tsh tcursor (DOT _ancestorsIdx) ((map (fun x => (rep_index (snd x)))  c) ++ idx_end) p * (* or its reverse? *)
   field_at Tsh tcursor (DOT _ancestors) ((map getval (map fst c)) ++ anc_end) p.
 
 Lemma cursor_rep_local_prop: forall c r p,
@@ -181,58 +173,58 @@ Hint Resolve cursor_rep_valid_pointer: valid_pointer.
 
 Inductive subnode {X:Type} : node X -> node X -> Prop :=
 | sub_refl: forall n, subnode n n
-| sub_ptr0: forall n le b x, subnode n (btnode X (Some n) le b x)
-| sub_entr: forall n p le b x k, subnode n (btnode X p (cons X (keychild X k n) le) b x)
-| sub_cons: forall n p le e b x, subnode n (btnode X p le b x) ->
-                                 subnode n (btnode X p (cons X e le) b x)
+| sub_ptr0: forall n le b First Last x, subnode n (btnode X (Some n) le b First Last x)
+| sub_entr: forall n p le b First Last x k, subnode n (btnode X p (cons X (keychild X k n) le) b First Last x)
+| sub_cons: forall n p le e b First Last x, subnode n (btnode X p le b First Last x) ->
+                                 subnode n (btnode X p (cons X e le) b First Last x)
 | sub_trans: forall n n1 n2, subnode n n1 -> subnode n1 n2 -> subnode n n2.
 
 
-Lemma btnode_rep_simpl_ptr0: forall le b x (p0:option (node val)) le0 b0 x0 proot p0,
-    btnode_rep (btnode val (Some (btnode val p0 le0 b0 x0)) le b x) proot =
-    !!(x=proot) &&
-      malloc_token Tsh tbtnode proot *
-    field_at Tsh tbtnode (DOT _numKeys) (Vint(Int.repr (Z.of_nat (numKeys_le le)))) proot *
-    field_at Tsh tbtnode (DOT _isLeaf) (Val.of_bool b) proot *
-    field_at Tsh tbtnode (DOT _ptr0) x0 proot *
-    btnode_rep (btnode val p0 le0 b0 x0) x0 *
-    field_at Tsh tbtnode (DOT _entries) (le_to_list_complete le) proot *
-    le_iter_sepcon le.
-Proof.
-  intros. apply pred_ext; entailer!; simpl; entailer!.
-Qed.
+(* Lemma btnode_rep_simpl_ptr0: forall le b x (p0:option (node val)) le0 b0 x0 proot p0 First Last, *)
+(*     btnode_rep (btnode val (Some (btnode val p0 le0 b0 x0)) le b First Last x) proot = *)
+(*     !!(x=proot) && *)
+(*       malloc_token Tsh tbtnode proot * *)
+(*     field_at Tsh tbtnode (DOT _numKeys) (Vint(Int.repr (Z.of_nat (numKeys_le le)))) proot * *)
+(*     field_at Tsh tbtnode (DOT _isLeaf) (Val.of_bool b) proot * *)
+(*     field_at Tsh tbtnode (DOT _ptr0) x0 proot * *)
+(*     btnode_rep (btnode val p0 le0 b0 x0) x0 * *)
+(*     field_at Tsh tbtnode (DOT _entries) (le_to_list_complete le) proot * *)
+(*     le_iter_sepcon le. *)
+(* Proof. *)
+(*   intros. apply pred_ext; entailer!; simpl; entailer!. *)
+(* Qed. *)
 
-Lemma btnode_rep_simpl_keychild: forall ptr0 le b x proot k nptr0 nle nb nx,
-    btnode_rep (btnode val ptr0 (cons val (keychild val k (btnode val nptr0 nle nb nx)) le) b x) proot =
-    !!(x=proot) &&
-      malloc_token Tsh tbtnode proot *
-    field_at Tsh tbtnode (DOT _numKeys) (Vint(Int.repr (Z.of_nat (S (numKeys_le le))))) proot *
-    field_at Tsh tbtnode (DOT _isLeaf) (Val.of_bool b) proot *
-    match ptr0 with
-    | None => field_at Tsh tbtnode (DOT _ptr0) nullval proot
-    | Some n' => match n' with btnode _ _ _ p' => field_at Tsh tbtnode (DOT _ptr0) p' proot * btnode_rep n' p' end
-    end *
-    field_at Tsh tbtnode (DOT _entries) (le_to_list_complete (cons val (keychild val k (btnode val nptr0 nle nb nx)) le)) proot *
-    btnode_rep (btnode val nptr0 nle nb nx) nx *
-    le_iter_sepcon le.
-Proof.
-  intros. apply pred_ext; entailer!; simpl; entailer!.
-Qed.
+(* Lemma btnode_rep_simpl_keychild: forall ptr0 le b x proot k nptr0 nle nb nx, *)
+(*     btnode_rep (btnode val ptr0 (cons val (keychild val k (btnode val nptr0 nle nb nx)) le) b x) proot = *)
+(*     !!(x=proot) && *)
+(*       malloc_token Tsh tbtnode proot * *)
+(*     field_at Tsh tbtnode (DOT _numKeys) (Vint(Int.repr (Z.of_nat (S (numKeys_le le))))) proot * *)
+(*     field_at Tsh tbtnode (DOT _isLeaf) (Val.of_bool b) proot * *)
+(*     match ptr0 with *)
+(*     | None => field_at Tsh tbtnode (DOT _ptr0) nullval proot *)
+(*     | Some n' => match n' with btnode _ _ _ p' => field_at Tsh tbtnode (DOT _ptr0) p' proot * btnode_rep n' p' end *)
+(*     end * *)
+(*     field_at Tsh tbtnode (DOT _entries) (le_to_list_complete (cons val (keychild val k (btnode val nptr0 nle nb nx)) le)) proot * *)
+(*     btnode_rep (btnode val nptr0 nle nb nx) nx * *)
+(*     le_iter_sepcon le. *)
+(* Proof. *)
+(*   intros. apply pred_ext; entailer!; simpl; entailer!. *)
+(* Qed. *)
 
 Theorem subnode_rep: forall n root proot,
     subnode n root ->
     btnode_rep root proot |-- EX pn:val, btnode_rep n pn *
                               (btnode_rep n pn -* btnode_rep root proot).
 Proof.
-  intros.
-  induction H.
-  - Exists proot. cancel. rewrite <- wand_sepcon_adjoint. cancel.
-  - destruct n. Exists v. rewrite btnode_rep_simpl_ptr0 by auto.
-    entailer!. rewrite <- wand_sepcon_adjoint. entailer!.
-  - destruct n. Exists v. rewrite btnode_rep_simpl_keychild.
-    entailer!. rewrite <- wand_sepcon_adjoint. entailer!.
-  - admit.                      (* we can't use the induction hypothesis *)
-  - admit.                      (* same *)
+  (* intros. *)
+  (* induction H. *)
+  (* - Exists proot. cancel. rewrite <- wand_sepcon_adjoint. cancel. *)
+  (* - destruct n. Exists v. rewrite btnode_rep_simpl_ptr0 by auto. *)
+  (*   entailer!. rewrite <- wand_sepcon_adjoint. entailer!. *)
+  (* - destruct n. Exists v. rewrite btnode_rep_simpl_keychild. *)
+  (*   entailer!. rewrite <- wand_sepcon_adjoint. entailer!. *)
+  (* - admit.                      (* we can't use the induction hypothesis *) *)
+  (* - admit.                      (* same *) *)
 Admitted.
 
 Fixpoint cursor_correct {X:Type} (c:cursor X) (n:node X) (root:node X): Prop :=
@@ -241,7 +233,7 @@ Fixpoint cursor_correct {X:Type} (c:cursor X) (n:node X) (root:node X): Prop :=
   | (n',i)::c' => (cursor_correct c' n' root) /\ (nth_node i n' = Some n)
   end.
 
-Definition get_root {X:Type} (rel:relation X) : node X := fst (fst rel).
+Definition get_root {X:Type} (rel:relation X) : node X := fst(fst (fst rel)).
 
 Definition cursor_correct_rel {X:Type} (c:cursor X) (rel:relation X): Prop :=
   match c with
